src/FingerTreeInterface.v
@@ -17,69 +17,14 @@ Set Implicit Arguments.
 Set Contextual Implicit.
 Set Maximal Implicit Insertion.
 
-Definition a := nat.
+(* Auxiliaries for [approx_algebra] *)
 
-(** Operations symbols *)
-Inductive Op : Type :=
-| Empty
-| Cons (x : a)
-| Snoc (x : a)
-| Head
-| Tail
-| Append
-.
+Section AA.
 
-(* Pure reference implementation [eval_op_Seq] and cost specification [CostSpec_Seq] *)
-Section Seq.
-Import FingerTree.
-
-Definition Seq := FingerTree.Seq.
-
-Definition eval_op_Seq (o : Op) (vs : list (Seq a)) : list (Seq a) :=
-  match o, vs with
-  | Empty, _ => [Nil]
-  | Cons x, q :: _ => [cons x q]
-  | Snoc x, q :: _ => [snoc q x]
-  | Head, q :: _ => []  (* Doesn't create a new FT *)
-  | Tail, q :: _ => [tail q]
-  | Append, q :: q' :: _ => [append q q']
-  | _, _ => []
-  end.
-
-(* TODO: splitAt, as an example of operation with two outputs *)
-
-#[global] Instance PureImpl_Seq : PureImpl Op (Seq a) := eval_op_Seq.
-
-#[global] Instance CostSpec_Seq : CostSpec Op (Seq a) :=
-  fun o vs =>
-    match o, vs with
-    | (Empty | Cons _ | Snoc _ | Head | Tail), _ => 1
-    | Append, q :: q' :: _ => max (depth q) (depth q')
-    | _, _ => 0
-    end.
-
-End Seq.
-
-(* Clairvoyant translation *)
-Section SeqA.
+Notation Seq := FingerTree.Seq.
 Import FingerTreeM.
 
-Definition SeqA' := SeqA a.
-
-Definition exec_op_SeqA (o : Op) (vs : list SeqA') : M (list SeqA') :=
-  match o, vs with
-  | Empty, _ => ret [Nil]
-  | Cons x, q :: _ => let! q := consA (Thunk x) (Thunk q) in ret [q]
-  | Snoc x, q :: _ => let! q := snocA (Thunk q) (Thunk x) in ret [q]
-  | Head, q :: _ => let! _ := headA (Thunk q) in ret []  (* Doesn't create a new FT *)
-  | Tail, q :: _ => let! q := tailA (Thunk q) in ret [q]
-  | Append, q :: q' :: _ => let! q := appendA (Thunk q) (Thunk q') in ret [q]
-  | _, _ => ret []
-  end.
-
-#[global] Instance CvImpl_SeqA : CvImpl Op SeqA' := exec_op_SeqA.
-
-(** ** [ApproxOrder_Seq]: Order structure of [SeqA] *)
+Context {a : Type}.
 
 #[global] Instance Exact_Seq : Exact (Seq a) (SeqA a).
 Admitted.
@@ -93,14 +38,7 @@ Admitted.
 #[global] Instance Lub_SeqA : Lub (SeqA a). Admitted.
 #[global] Instance LubLaw_SeqA : LubLaw (SeqA a). Admitted.
 
-#[local] Instance exec_op_mon (o : Op) :
-  Morphisms.Proper (Morphisms.respectful less_defined less_defined)
-    (exec_op (op := Op) (valueA := SeqA') o).
-Proof.
-Admitted.
-
-
-#[global] Instance HasBottom_SeqA : HasBottom (SeqA a) := fun q =>
+#[global] Instance BottomOf_SeqA : BottomOf (SeqA a) := fun q =>
   match q with
   | Nil => Nil
   | Unit _ => Unit Undefined
@@ -110,28 +48,87 @@ Admitted.
 #[global] Instance BottomIsLeast_SeqA : BottomIsLeast (SeqA a).
 Admitted.
 
-#[global] Instance ApproxOrder_Seq : ApproxOrder Op (Seq a) SeqA'.
+End AA.
+
+(**)
+
+Definition a := nat.
+Definition value := FingerTree.Seq a.
+Definition valueA := FingerTreeM.SeqA a.
+Notation stack := (list value) (only parsing).
+Notation stackA := (list valueA) (only parsing).
+
+(** Operations symbols *)
+Inductive op : Type :=
+| Empty
+| Cons (x : a)
+| Snoc (x : a)
+| Head
+| Tail
+| Append
+.
+
+Import FingerTree.
+
+Definition eval : Eval op value :=
+  fun (o : op) (args : list value) => match o, args with
+  | Empty, _ => [Nil]
+  | Cons x, q :: _ => [cons x q]
+  | Snoc x, q :: _ => [snoc q x]
+  | Head, q :: _ => []  (* Doesn't create a new FT *)
+  | Tail, q :: _ => [tail q]
+  | Append, q :: q' :: _ => [append q q']
+  | _, _ => []
+  end.
+
+Definition budget : Budget op value :=
+  fun (o : op) (args : list value) => match o, args with
+  | (Empty | Cons _ | Snoc _ | Head | Tail), _ => 1
+  | Append, q :: q' :: _ => max (depth q) (depth q')
+  | _, _ => 0
+  end.
+
+Import FingerTreeM.
+
+Definition exec : Exec op valueA :=
+  fun (o : op) (args : list valueA) => match o, args with
+  | Empty, _ => ret [Nil]
+  | Cons x, q :: _ => let! q := consA (Thunk x) (Thunk q) in ret [q]
+  | Snoc x, q :: _ => let! q := snocA (Thunk q) (Thunk x) in ret [q]
+  | Head, q :: _ => let! _ := headA (Thunk q) in ret []  (* Doesn't create a new FT *)
+  | Tail, q :: _ => let! q := tailA (Thunk q) in ret [q]
+  | Append, q :: q' :: _ => let! q := appendA (Thunk q) (Thunk q') in ret [q]
+  | _, _ => ret []
+  end.
+
+#[export] Existing Instances eval budget exec.
+
+Lemma monotonic_exec (o : op) : Monotonic (exec o).
 Proof.
-  econstructor; try typeclasses eauto.
-Defined.
-
-(** * Main theorem: HasAmortizedCost_Seq *)
-
-#[global] Instance Potential_SeqA : Potential SeqA' := fun t =>
-  0 (* TODO *).
-
-#[global] Instance HasPotential_SeqA : HasPotential SeqA'.
 Admitted.
 
-#[global] Instance MonotoneCvImpl_SeqA : MonotoneCvImpl CvImpl_SeqA.
-Admitted.
+Definition approx_algebra : ApproxAlgebra value valueA.
+Proof. econstructor; try typeclasses eauto. Defined.
+#[export] Existing Instance approx_algebra.
 
-#[global] Instance Physicist'sArgument_SeqA : Physicist'sArgument CostSpec_Seq CvImpl_SeqA.
-Proof.
-  econstructor.
-Admitted.
+Lemma well_defined_exec : WellDefinedExec.
+Proof. constructor; exact monotonic_exec. Qed.
+#[export] Existing Instance well_defined_exec.
 
-Theorem HasAmortizedCost_Seq : HasAmortizedCost CostSpec_Seq CvImpl_SeqA.
+(* "debt" in BankersQueue *)
+Definition potential : Potential valueA := (* ... *)
+  fun t => _depthX t.
+#[export] Existing Instance potential.
+
+Lemma well_defined_potential : WellDefinedPotential.
+Proof. Admitted.
+#[export] Existing Instance well_defined_potential.
+
+Theorem physicist's_argument : Physicist'sArgument.
 Proof.
-  apply physicist's_method.
-Qed.
+  red.
+Admitted.
+#[export] Existing Instance physicist's_argument.
+
+Theorem amortized_cost : AmortizedCostSpec.
+Proof. apply physicist's_method. Qed.
