src/Interfaces.v
@@ -8,9 +8,22 @@ Import ListNotations.
 From Clairvoyance Require Import Core Approx ApproxM List Misc Cost.
 
 Set Primitive Projections.
-(* Set Implicit Arguments.
-Set Contextual Implicit.
-Set Maximal Implicit Insertion. *)
+
+(* * Preamble: miscellaneous definitions *)
+
+(** Order structure on approximation values [valueA].
+    Core operations ([exact], [less_defined], [lub], [bottom_of])
+    and their properties. *)
+Class ApproxAlgebra (t tA : Type) : Type :=
+  { AO_Exact         :> Exact t     tA
+  ; AO_LessDefined   :> LessDefined tA
+  ; AO_Lub           :> Lub         tA
+  ; AO_BottomOf      :> BottomOf    tA
+
+  ; AO_PreOrder      :> PreOrder (less_defined (a := tA))
+  ; AO_LubLaw        :> LubLaw        tA
+  ; AO_BottomIsLeast :> BottomIsLeast tA
+  }.
 
 (* lookups xs [n; m; p] = [xs!!n; xs!!m; xs!!p], or None if out of bounds *)
 Fixpoint lookups {A} (xs : list A) (ns : list nat) : option (list A) :=
@@ -21,213 +34,22 @@ Fixpoint lookups {A} (xs : list A) (ns : list nat) : option (list A) :=
     option_map (cons x) (lookups xs ns))
   end.
 
-Class PureImpl (op value : Type) : Type :=
-  eval_op : op -> list value -> list value.
+Definition Monotonic {a b} `{LessDefined a, LessDefined b} (f : a -> b) : Prop :=
+  forall x y, x `less_defined` y -> f x `less_defined` f y.
 
-Definition event (op : Type) : Type := (op * list nat).
-Definition trace (op : Type) : Type := list (event op).
-Notation stack := list (only parsing).
-
-Section Pure.
-
-Context {op value : Type} {pure_impl : PureImpl op value}.
-
-Definition eval_event '((o, ns) : event op) (vs : stack value) : stack value :=
-  match lookups vs ns with
-  | None => vs  (* noop *)
-  | Some xs => vs ++ eval_op o xs
-  end.
-
-Fixpoint eval_trace_from (es : trace op) (xs : stack value) : stack value :=
-  match es with
-  | [] => xs
-  | e :: es => eval_trace_from es (eval_event e xs)
-  end.
-
-Definition eval_trace (es : trace op) : stack value := eval_trace_from es [].
-
-End Pure.
-
-(* The cost may depend on the input *)
-Class CostSpec (op value : Type) : Type :=
-  cost_op : op -> list value -> nat.
-
-Section Cost.
-
-Context {op value : Type} {pure_impl : PureImpl op value} {cost_spec : CostSpec op value}.
-
-Definition cost_event '((o, ns) : event op) (vs : stack value) : nat :=
-  match lookups vs ns with
-  | None => 0
-  | Some xs => cost_op o xs
-  end.
-
-Fixpoint cost_trace_from (es : trace op) (vs : stack value) : nat :=
-  match es with
-  | [] => 0
-  | e :: es => cost_event e vs + cost_trace_from es (eval_event e vs)
-  end.
-
-Definition cost_trace (es : trace op) : nat := cost_trace_from es [].
-
-End Cost.
-
-Class CvImpl (op valueA : Type) : Type :=
-  exec_op : op -> list valueA -> M (list valueA).
-
-Section Cv.
-
-Context {op valueA : Type} {cv_impl : CvImpl op valueA}.
-
-Definition exec_event '((o, ns) : event op) (vs : stack valueA) : M (stack valueA) :=
-  match lookups vs ns with
-  | None => ret vs  (* noop *)
-  | Some xs => let! ys := exec_op o xs in ret (vs ++ ys)
-  end.
-
-Fixpoint exec_trace_from (es : trace op) (vs : stack valueA) : M (stack valueA) :=
-  match es with
-  | [] => ret vs
-  | e :: es => let! vs := exec_event e vs in exec_trace_from es vs
-  end.
-
-Definition exec_trace (es : trace op) : M (stack valueA) :=
-  exec_trace_from es [].
-
-End Cv.
-
-(** Order structure on approximation values [valueA].
-    Core operations ([exact], [less_defined], [lub], [bottom_of])
-    and their properties. *)
-Class ApproxOrder (op value valueA : Type) : Type :=
-  { AO_Exact :> Exact value valueA
-  ; AO_LessDefined :> LessDefined valueA
-  ; AO_PreOrder :> PreOrder (less_defined (a := valueA))
-  ; AO_Lub :> Lub valueA
-  ; AO_LubLaw :> LubLaw valueA
-  ; AO_HasBottom :> HasBottom valueA
-  ; AO_BottomIsLeast :> BottomIsLeast valueA
-  }.
-
-(* Monotonicity of [exec_op] *)
-Class MonotoneCvImpl {op value valueA}
-    {approx_order : ApproxOrder op value valueA}
-    (cv_impl : CvImpl op valueA) : Prop :=
-  exec_op_mon : forall o, Proper (less_defined ==> less_defined) (exec_op (valueA := valueA) o).
-
-(** Amortized cost specification. *)
-Section HasAmortizedCost.
-
-Context {op value valueA : Type}
-  {pure_impl : PureImpl op value}
-  {cost_spec : CostSpec op value}
-  {cv_impl : CvImpl op valueA}.
-
-(** The cost of executing the whole trace is less than
-    its aggregated bound. *)
-Definition HasAmortizedCost : Prop :=
-  forall os : trace op,
-    (cost_of (exec_trace os) <= cost_trace os)%NAT.
-
-(** Equivalent formulation as a weakest precondition. *)
-Definition HasAmortizedCost' : Prop :=
-  forall os : trace op,
-    exec_trace os [[ fun _ c => c <= cost_trace os ]].
-
-Context
-  {approx_order : ApproxOrder op value valueA}.
-
-Theorem has_amortized_cost' :
-  HasAmortizedCost <-> HasAmortizedCost'.
-Admitted.
-
-End HasAmortizedCost.
-
-Arguments HasAmortizedCost : clear implicits.
-Arguments HasAmortizedCost {op value valueA pure_impl} cost_spec cv_impl.
-
-Arguments HasAmortizedCost' : clear implicits.
-Arguments HasAmortizedCost' {op value valueA pure_impl} cost_spec cv_impl.
-
-(** Clairvoyant Physicist's method *)
-
-(* TODO: These classes are a bit of a mess. Find a good way to package all of the required operations and facts together. *)
-
-Class Potential (a : Type) : Type :=
-  potential : a -> nat.
-
-Definition sumof {A} (f : A -> nat) : list A -> nat :=
+Definition sumof {a} (f : a -> nat) : list a -> nat :=
   fold_right (fun x s => f x + s) 0.
 
-#[global]
-Instance Potential_list {a} `{Potential a} : Potential (list a) := sumof potential.
-
-Class PotentialLub (a : Type) `{Potential a, LessDefined a, Lub a} : Prop :=
-  potential_lub : forall x y : a, cobounded x y -> potential (lub x y) <= potential x + potential y.
-
-#[global]
-Instance PotentialLub_list {a} `{PotentialLub a} : PotentialLub (list a).
-Proof.
-  intros x y.
-  induction 1 as [ | ? ? ? ? ? ? IH ] using cobounded_list_ind;
-    cbn; [ reflexivity | ].
-  rewrite IH, potential_lub by assumption.
-  clear. generalize (potential x) (potential y). lia.
-Qed.
-
-Lemma potential_app {a} `{Potential a} (x y : list a)
-  : potential (x ++ y) = potential x + potential y.
+Lemma sumof_app {a} (f : a -> nat)  (x y : list a) : sumof f (x ++ y) = sumof f x + sumof f y.
 Proof.
   induction x as [ | x0 ? IH ]; cbn; [ auto | rewrite IH ]. lia.
 Qed.
 
-Class PotentialBottom (a : Type) `{Potential a, HasBottom a} : Prop :=
-  potential_bottom : forall x : a, potential (bottom_of x) = 0.
+Definition SubadditiveMeasure {a : Type} (f : a -> nat) `{LessDefined a, Lub a} : Prop :=
+  forall x y : a, cobounded x y -> f (lub x y) <= f x + f y.
 
-#[global] Instance PotentialBottom_list {a} `{PotentialBottom a} : PotentialBottom (list a).
-Proof.
-  intros x; induction x as [ | ? ? IH ]; cbn; [ reflexivity | ].
-  rewrite potential_bottom, IH. reflexivity.
-Qed.
-
-Class HasPotential {op value} valueA
-    {approx_order : ApproxOrder op value valueA} : Type :=
-  { _Potential :> Potential valueA
-  ; _PotentialLub :> PotentialLub valueA
-  ; _PotentialBottom :> PotentialBottom valueA
-  }.
-
-Section Physicist'sArgument.
-
-Context {op value valueA : Type}
-  {approx_order : ApproxOrder op value valueA}
-  {pure_impl : PureImpl op value}
-  {cost_spec : CostSpec op value}
-  {cv_impl : CvImpl op valueA}.
-
-(** Theorem statement: "the implementation [cv_impl] simulates [pure_impl]
-    with amortized cost bounded above by [cost_spec] plus a potential
-    difference." *)
-(* Note: lazy evaluation works backwards.
-   We are first given an [output] demand,
-   obtained as an approximation of the reference output via [eval_op],
-   and we have to find a matching [input] demand. *)
-Class Physicist'sArgument : Type :=
-  { for_some_potential :> HasPotential valueA
-  ; exec_cost : forall (o : op) (vs : list value),
-      forall output : stack valueA, output `is_approx` eval_op o vs ->
-      exists input : stack valueA, input `is_approx` vs /\
-      exec_op o input [[ fun r c =>
-        output `less_defined` r /\
-        potential input + c <= cost_op o vs + potential output ]]
-  }.
-
-End Physicist'sArgument.
-
-Arguments Physicist'sArgument : clear implicits.
-Arguments Physicist'sArgument {op value valueA approx_order pure_impl} cost_spec cv_impl.
-
-(* Auxiliary lemmas *)
+Definition ZeroMeasure {a : Type} (f : a -> nat) `{BottomOf a} : Prop :=
+  forall x, f (bottom_of x) = 0.
 
 Lemma less_defined_lookups {a aA} {EE : Exact a aA} {LD : LessDefined aA}
     {f : aA -> nat} {ns : list nat} {xs ys : list a}
@@ -276,54 +98,6 @@ Proof.
     rewrite Hlub; cbn. reflexivity.
 Qed.
 
-Section Soundness.
-
-Context {op value valueA : Type}
-  {approx_order : ApproxOrder op value valueA}
-  {pure_impl : PureImpl op value}
-  {cost_spec : CostSpec op value}
-  {cv_impl : CvImpl op valueA}
-  {monotone_cv_impl : MonotoneCvImpl cv_impl}
-  {pa : Physicist'sArgument cost_spec cv_impl}.
-
-Lemma exec_cost_event (e : event op) (vs : stack value) output
-  : output `is_approx` eval_event e vs ->
-    exists input, input `is_approx` vs /\
-    exec_event e input [[ fun r c =>
-      output `less_defined` r /\
-      potential input + c <= cost_event e vs + potential output ]].
-Proof.
-  destruct e as [o ns].
-  unfold eval_event, exec_event.
-  destruct (lookups vs ns) eqn:E; intros Hout.
-  - rewrite exact_list_app in Hout. apply less_defined_app_inv in Hout.
-    destruct Hout as (out1 & out2 & Hout & Hout1 & Hout2).
-    apply exec_cost in Hout2. destruct Hout2 as (input & Hin & HH).
-    destruct (less_defined_lookups (f := potential) E _ Hin) as (input' & Hin' & Hpotential & HH'); change (sumof (A := valueA) potential) with (potential (a := list valueA)) in Hpotential.
-    exists (lub input' out1).
-    split; [ apply lub_least_upper_bound; auto | ].
-    destruct (lookups_lub (ys := out1) HH') as (y1 & Hx & Hcob1 & Hy);
-      [ eauto | ].
-    rewrite Hy.
-    mgo_. relax; [ | intros ? ? Hr; mgo_; rewrite Nat.add_0_r; exact Hr ].
-    eapply optimistic_corelax;
-      [ eapply exec_op_mon, lub_upper_bound_l; eauto | | ].
-    { unfold uc; intros * ? ? []; split.
-      - rewrite H1. apply less_defined_app; reflexivity + assumption.
-      - rewrite <- H2. lia. }
-    relax; [ apply HH | cbn; intros r c [Hr Hc] ].
-    split; [ rewrite Hout; apply less_defined_app; [ apply lub_upper_bound_r; eauto | assumption ] | ].
-    rewrite potential_lub by eauto. rewrite Hout, potential_app.
-    rewrite E, Hpotential.
-    revert Hc. generalize (cost_op o l). lia.
-  - exists output. rewrite (less_defined_lookups_None E Hout).
-    split; [ auto | ]. mgo_. split; [ reflexivity | lia ].
-Qed.
-
-Lemma eval_trace_from_mon os : Proper (less_defined ==> less_defined) (exec_trace_from os).
-Proof.
-Admitted.
-
 Notation pr := (pointwise_relation _).
 
 Lemma uc_ext {a} `{LessDefined a} : Proper (pr (pr eq) ==> iff) (uc (a := a)).
@@ -333,46 +107,244 @@ Proof.
   rewrite <- Hf. apply Hg.
 Qed.
 
+(** * General interface for lazy data structures *)
+
+Section Interface.
+
+Context {op value valueA : Type}.
+Context {approx_algebra : ApproxAlgebra value valueA}.
+
+Definition Eval : Type := op -> list value -> list value.
+Existing Class Eval.
+
+Context {eval : Eval}.
+
+Definition event : Type := (op * list nat).
+Definition trace : Type := list event.
+Notation stack := (list value) (only parsing).
+Notation stackA := (list valueA) (only parsing).
+
+Definition eval_event '((o, ns) : event) (vs : stack) : stack :=
+  match lookups vs ns with
+  | None => vs  (* noop *)
+  | Some xs => vs ++ eval o xs
+  end.
+
+Fixpoint eval_trace_from (es : trace) (xs : stack) : stack :=
+  match es with
+  | [] => xs
+  | e :: es => eval_trace_from es (eval_event e xs)
+  end.
+
+Definition eval_trace (es : trace) : stack := eval_trace_from es [].
+
+(* The cost may depend on the input *)
+Definition Budget : Type := op -> list value -> nat.
+Existing Class Budget.
+
+Context {budget : Budget}.
+
+Definition budget_event '((o, ns) : event) (vs : stack) : nat :=
+  match lookups vs ns with
+  | None => 0
+  | Some xs => budget o xs
+  end.
+
+Fixpoint budget_trace_from (es : trace) (vs : stack) : nat :=
+  match es with
+  | [] => 0
+  | e :: es => budget_event e vs + budget_trace_from es (eval_event e vs)
+  end.
+
+Definition budget_trace (es : trace) : nat := budget_trace_from es [].
+
+Definition Exec : Type := op -> list valueA -> M (list valueA).
+Existing Class Exec.
+
+Context {exec : Exec}.
+
+Definition exec_event '((o, ns) : event) (vs : stackA) : M (stackA) :=
+  match lookups vs ns with
+  | None => ret vs  (* noop *)
+  | Some xs => let! ys := exec o xs in ret (vs ++ ys)
+  end.
+
+Fixpoint exec_trace_from (es : trace) (vs : stackA) : M (stackA) :=
+  match es with
+  | [] => ret vs
+  | e :: es => let! vs := exec_event e vs in exec_trace_from es vs
+  end.
+
+Definition exec_trace (es : trace) : M (stackA) :=
+  exec_trace_from es [].
+ 
+Class WellDefinedExec : Prop :=
+  { monotonic_exec : forall o, Monotonic (exec o)
+  }.
+
+Context {wd_exec : WellDefinedExec}.
+
+Lemma exec_trace_from_mon os : Proper (less_defined ==> less_defined) (exec_trace_from os).
+Proof.
+Admitted.
+
+(** Amortized cost specification. *)
+Section AmortizedCostSpec.
+
+(** The cost of executing the whole trace is less than
+    its aggregated bound. *)
+Definition AmortizedCostSpec : Prop :=
+  forall os : trace, (cost_of (exec_trace os) <= budget_trace os)%NAT.
+
+(** Equivalent formulation as a weakest precondition. *)
+Definition AmortizedCostSpec' : Prop :=
+  forall os : trace, exec_trace os [[ fun _ c => c <= budget_trace os ]].
+
+Theorem has_amortized_cost' :
+  AmortizedCostSpec <-> AmortizedCostSpec'.
+Admitted.
+
+End AmortizedCostSpec.
+
+(** Clairvoyant Physicist's method *)
+
+(* TODO: These classes are a bit of a mess. Find a good way to package all of the required operations and facts together. *)
+
+Definition Potential : Type := valueA -> nat.
+Existing Class Potential.
+
+Context {potential : Potential}.
+
+Class WellDefinedPotential : Prop :=
+  { potential_lub    : SubadditiveMeasure potential
+  ; potential_bottom : ZeroMeasure potential
+  }.
+
+Context {wd_potential : WellDefinedPotential}.
+
+Lemma potential_lub_list (potential_lub : SubadditiveMeasure potential) : SubadditiveMeasure (sumof potential).
+Proof.
+  intros x y.
+  induction 1 as [ | ? ? ? ? ? ? IH ] using cobounded_list_ind;
+    cbn; [ reflexivity | ].
+  rewrite IH, potential_lub by assumption.
+  clear. generalize (potential x) (potential y). lia.
+Qed.
+
+Lemma potential_lub_list_ : SubadditiveMeasure (sumof potential).
+Proof. exact (potential_lub_list potential_lub). Qed.
+
+Lemma potential_bottom_list (potential_bottom : ZeroMeasure potential) : ZeroMeasure (sumof potential).
+Proof.
+  intros x; induction x as [ | ? ? IH ]; cbn; [ reflexivity | ].
+  rewrite potential_bottom, IH. reflexivity.
+Qed.
+
+Lemma potential_bottom_list_ : ZeroMeasure (sumof potential).
+Proof. exact (potential_bottom_list potential_bottom). Qed.
+
+(** Theorem statement: "the implementation [exec] simulates [_eval]
+    with amortized cost bounded above by [budget] plus a potential
+    difference." *)
+(* Note: lazy evaluation works backwards.
+   We are first given an [output] demand,
+   obtained as an approximation of the reference output via [eval_op],
+   and we have to find a matching [input] demand. *)
+Definition Physicist'sArgument : Prop :=
+  forall (o : op) (vs : list value),
+    forall output : stackA, output `is_approx` eval o vs ->
+    exists input : stackA, input `is_approx` vs /\
+    exec o input [[ fun r c =>
+      output `less_defined` r /\
+      sumof potential input + c <= budget o vs + sumof potential output ]].
+Existing Class Physicist'sArgument.
+
+Context {exec_cost : Physicist'sArgument}.
+
+Section Soundness.
+
+Lemma exec_event_cost (e : event) (vs : stack) output
+  : output `is_approx` eval_event e vs ->
+    exists input, input `is_approx` vs /\
+    exec_event e input [[ fun r c =>
+      output `less_defined` r /\
+      sumof potential input + c <= budget_event e vs + sumof potential output ]].
+Proof.
+  destruct e as [o ns].
+  unfold eval_event, exec_event.
+  destruct (lookups vs ns) eqn:E; intros Hout.
+  - rewrite exact_list_app in Hout. apply less_defined_app_inv in Hout.
+    destruct Hout as (out1 & out2 & Hout & Hout1 & Hout2).
+    apply exec_cost in Hout2. destruct Hout2 as (input & Hin & HH).
+    destruct (less_defined_lookups (f := potential) E _ Hin) as (input' & Hin' & Hpotential & HH').
+    exists (lub input' out1).
+    split; [ apply lub_least_upper_bound; auto | ].
+    destruct (lookups_lub (ys := out1) HH') as (y1 & Hx & Hcob1 & Hy);
+      [ eauto | ].
+    rewrite Hy.
+    mgo_. relax; [ | intros ? ? Hr; mgo_; rewrite Nat.add_0_r; exact Hr ].
+    eapply optimistic_corelax;
+      [ eapply monotonic_exec, lub_upper_bound_l; eauto | | ].
+    { unfold uc; intros * ? ? []; split.
+      - rewrite H1. apply less_defined_app; reflexivity + assumption.
+      - rewrite <- H2. lia. }
+    relax; [ apply HH | cbn; intros r c [Hr Hc] ].
+    split; [ rewrite Hout; apply less_defined_app; [ apply lub_upper_bound_r; eauto | assumption ] | ].
+    rewrite potential_lub_list_ by eauto. rewrite Hout, sumof_app.
+    rewrite E, Hpotential.
+    revert Hc. generalize (budget o l). lia.
+  - exists output. rewrite (less_defined_lookups_None E Hout).
+    split; [ auto | ]. mgo_. split; [ reflexivity | lia ].
+Qed.
+
 Lemma physicist's_method_aux
-  : forall (os : trace op) (vs : list value),
+  : forall (os : trace) (vs : list value),
     forall output, output `is_approx` eval_trace_from os vs ->
     exists input, input `is_approx` vs /\
       exec_trace_from os input [[ fun r c =>
-        output `less_defined` r /\ potential input + c <= cost_trace_from os vs + potential output ]].
+        output `less_defined` r /\ sumof potential input + c <= budget_trace_from os vs + sumof potential output ]].
 Proof.
   induction os as [ | [o ns] os IH ]; intros vs output Hout; cbn.
   - exists output. split; [apply Hout | ].
     apply optimistic_ret. split; [ reflexivity | lia ].
   - cbn in Hout. specialize (IH (eval_event (o, ns) vs) output Hout).
     destruct IH as (input & Hin & IH).
-    destruct (exec_cost_event _ _ _ Hin) as (inp & Hinp & HH).
+    destruct (exec_event_cost _ _ _ Hin) as (inp & Hinp & HH).
     exists inp. split; [ auto | ].
     mgo_. relax; [ apply HH | cbn; intros ? ? [HI HJ] ].
-    eapply optimistic_corelax; [ apply eval_trace_from_mon; eassumption | | ].
+    eapply optimistic_corelax; [ apply exec_trace_from_mon; eassumption | | ].
     { eapply uc_ext; [ intros ? ?; rewrite Nat.add_assoc; reflexivity | apply uc_acost ]. }
     relax; [ apply IH | cbn; intros ? ? [HK HL] ].
     split; [ auto | ].
     lia.
 Qed.
 
-Theorem physicist's_method : HasAmortizedCost cost_spec cv_impl.
+Theorem physicist's_method : AmortizedCostSpec.
 Proof.
   apply has_amortized_cost'.
   intros os. destruct (physicist's_method_aux os [] (bottom_of (exact (eval_trace_from os [])))) as (d0 & Hd0 & HH).
   { apply bottom_is_least. }
   inversion Hd0; clear Hd0; subst.
   apply (optimistic_mon HH); cbn.
-  intros ? ? [_ INEQ]. fold (cost_trace os) in INEQ.
-  rewrite potential_bottom, Nat.add_0_r in INEQ.
+  intros ? ? [_ INEQ]. fold (budget_trace os) in INEQ.
+  rewrite potential_bottom_list_, Nat.add_0_r in INEQ.
   exact INEQ.
 Qed.
 
 End Soundness.
 
+End Interface.
+
+Arguments Eval : clear implicits.
+Arguments Budget : clear implicits.
+Arguments Exec : clear implicits.
+Arguments ApproxAlgebra : clear implicits.
+Arguments Potential : clear implicits.
+
 (*
 Section RealTimeCost.
 
-Context {op : Type} (j : CostSpec op) (j' : St.Impl op).
+Context {op : Type} (j : Budget op) (j' : St.Impl op).
 
 Notation op' := (op * list nat)%type.
 
@@ -387,7 +359,7 @@ Definition RealTimeCost : Prop :=
 End RealTimeCost.
 
 Definition ImplRealTimeCost
-    (op : Type) (j : CostSpec op) (j' : Cv.Impl op) {AO : ApproxOrder j j'}
+    (op : Type) (j : Budget op) (j' : Cv.Impl op) {AO : ApproxAlgebra j j'}
   : Prop :=
   forall (os : list (op * list nat)) (o : op) (ns : list nat),
     ( cost_of (exec_trace (j := j') (os ++ [(o, ns)]) [])
